\chapter{Анализ внутренних силовых факторов}

\section{Задача 1}

$ \sum P_x = 0 $

$ R_A - q \cdot \frac{2L}{3} = 0 $

$ R_A = \frac{2}{3} \left(qL\right) = \frac{2}{3} P $

\vspace{1.5ex}

Участок 1 $ \left(0 \le x_1 < \frac{L}{3}\right) $

$ \sum P_{x_1} = 0 $

$ N_1 + R_A = 0 $

$ N_1 = -R_A = -\frac{2}{3} P $

\vspace{1.5ex}

Участок 2 $ \left(\frac{L}{3} \le x_2 < L\right) $

$ \sum P_{x_2} = 0 $

$ N_2 + R_A - q \left(x_2 - \frac{L}{3}\right) = 0 $

$ N_2 = -\frac{2}{3} P $

При $ x_2 = \frac{L}{3} $: $ N_2 = -R_A = -R_A = -\frac{2}{3} P $.

При $ x_2 = L $:           $ N_2 = 0 $.


\section{Задача 2}

$ \sum P_x = 0 $

$ R_A - q \cdot \frac{2L}{3} = 0 $

$ R_A = \frac{2}{3} \left(qL\right) = \frac{2}{3} P $

\vspace{1.5ex}

Участок 1 $ \left(0 \le x_1 < \frac{L}{3}\right) $

$ \sum P_{x_1} = 0 $

$ N_1 + R_A = 0 $

$ N_1 = -R_A = -\frac{2}{3} P $

\vspace{1.5ex}

Участок 2 $ \left(\frac{L}{3} \le x_2 < L\right) $

$ \sum P_{x_2} = 0 $

$ N_2 + R_A - q \left(x_2 - \frac{L}{3}\right) = 0 $

$ N_2 = -\frac{2}{3} P $

При $ x_2 = \frac{L}{3} $: $ N_2 = -R_A = -R_A = -\frac{2}{3} P $.

При $ x_2 = L $:           $ N_2 = 0 $.

\section{Задача 3}

$ \sum P_x = 0 $

$ 2P - q \cdot \left(2L\right) + P - P = 0 $

\vspace{1.5ex}

Участок 1. $ 0 \le x < 2L $

$ P_x = 0 $

$ 2P - qx + N_1 = 0 $

$ N_1 = qx - 2P $

\vspace{1.5ex}

Участок 2. $ 2L \le x_2 < 3L $

$ \sum P_x = 0 $

$ 2P - q \cdot \left(2L\right) + P + N_2 = 0 $

$ N_2 = -P $


\section{Задача 4}

$ \sum M_x = M_A - \left(2m\right) \cdot \frac{L}{2} = 0 $,
откуда $ M_A = \left(2m\right) \cdot \frac{L}{2} = mL =  M $.

\vspace{1.5ex}

Участок 1 $ \left(0 \le x < \frac{L}{2}\right) $

$ \sum M_x = M_A + M_1 = 0 $,
откуда $ M_1 = -M_A = -M $

\vspace{1.5ex}

Участок 2 $ \left(\frac{L}{2} \le x < L\right) $

$ \sum M_x = M_A + M_2 - 2m \cdot \left(x - \frac{L}{2}\right) = 0 $,
откуда $ M_2 = 2m \cdot \left(x - \frac{L}{2}\right) - M_A = 2mx - mL - M = 2mx - 2M $


\section{Задача 5}

$ \sum M_x = -3M + 2mL + mL = 0 $.

\vspace{1.5ex}

Участок 1 $ \left(0 \le x < L\right) $

$ \sum M_x = -3M + M_1 = 0 $,
откуда $ M_1 = 3M $.

\vspace{1.5ex}

Участок 2 $ \left(L \le x < 2L\right) $

$ \sum M_x = -3M + 2m \cdot \left(x- L\right) + M_2 =  0 $,
откуда $ M_2 = 3M - 2m \cdot \left(x - L\right) = -2mx + 3M + 2mL = -2mx + 5M $.

\vspace{1.5ex}

Участок 3 $ \left(2L \le x < 3L\right) $

$ \sum M_x = -3M + 2mL + m \cdot \left(x- 2L\right) + M_3 =  0 $,
откуда $ M_2 = 3M - 2mL - m \cdot \left(x - 2L\right) = 3M - 2mL - mx + 2mL = -mx + 3M $.


\section{Задача 6}
ПРОВЕРИТЬ ЭТУ ЗАДАЧУ. ОНА НЕПРАВИЛЬНАЯ С ВЕРОЯТНОСТЬЮ 146 \%

$ \sum M_x = M_A - 3P \cdot L + P \cdot 2L = 0 $,
    откуда $ M_A = 3PL - 2PL = PL $.

$ \sum P_x = R_A - 3P + P = 0 $,
откуда $ R_A = 3P - P = 2P $.

\vspace{1.5ex}

Участок 1 $ \left(0 \le x < L\right) $

$ \sum M_x = M_A + M_1 = 0 $,
откуда $ M_1 = -M_A = -PL $.

$ \sum P_x = R_A - Q_x = 0 $,
откуда $ Q_x = R_A = 2P $.

\vspace{1.5ex}

Участок 2 $ \left(L \le x < 2L\right) $

$ \sum M_x = M_A - PL + M_2 = 0 $,
откуда $ M_2 = -M_A + PL = PL + PL = 2PL $.

$ \sum P_x = R_A - 3P - Q_x = 0 $,
откуда $ Q_x = R_A - 3P = 2P - 3P = -P $.


\section{Задача 7}

$ \sum M_A = -Pa - P \cdot 2a + R_B \cdot 3a - P \cdot 4a = 0 $,
откуда $ R_B = \frac{1}{3a} \cdot \left(Pa + 2Pa + 4Pa\right) = \frac{7}{3}P $.

$ \sum M_B = R_A \cdot 3a + P \cdot 2a + Pa - Pa = 0 $,
откуда $ R_A = \frac{1}{3a} \left(2Pa + Pa - Pa\right) = \frac{2}{3}P $.

$ \sum P_y = R_A - P - P + R_B - P = \frac{2}{3}P + \frac{7}{3} - 3P = 0 $.

\vspace{1.5ex}

Участок 1 $ \left(0 \le x < a\right) $

$ \sum P_{y_1} = R_A - Q_1 = 0 $,
откуда $ Q_1 = R_A = \frac{2}{3}P $.

$ \sum M_{O_1} = -R_A x + M_1 = 0 $,
откуда $ M_1 = R_A x = \frac{2}{3} Px $.

\vspace{1.5ex}

Участок 2 $ \left(a \le x < 2a\right) $

$ \sum P_{y_2} = R_A - P - Q_2 = 0 $,
откуда $ Q_2 = R_A - P = \frac{2}{3}P - P = -\frac{1}{3}P$.

$ \sum M_{O_2} = -R_A x + P \cdot (x - a) + M_2 = 0 $,
откуда $ M_2 = R_A x - P \cdot (x - a) = \frac{2}{3}Px - Px + Pa = -\frac{1}{3}Px + Pa $.

\vspace{1.5ex}

Участок 3 $ \left(2a \le x < 3a\right) $

$ \sum P_{y_3} = R_A - P - P - Q_3 = 0 $,
откуда $ Q_3 = R_A - P - P = \frac{2}{3}P - 2P = -\frac{4}{3}P$.

$ \sum M_{O_3} = -R_A x + P \cdot (x - a) + P \cdot (x - 2a) + M_3 = 0 $,
откуда $ M_3 = R_A x - P \cdot (x - a) - P \cdot (x - 2a) = \frac{2}{3}Px - Px + Pa - Px + 2Pa = -\frac{4}{3}Px + 3Pa $.

\vspace{1.5ex}

Участок 4 $ \left(3a \le x < 4a\right) $

$ \sum P_{y_4} = R_A - P - P + R_B - Q_4 = 0 $,
откуда $ Q_4 = R_A - P - P + R_B = \frac{2}{3}P - 2P + \frac{7}{3}P = P $.

$ \sum M_{O_4} = -R_A x + P \cdot (x - a) + P \cdot (x - 2a) - R_B \cdot (x - 3a) + M_4 = 0 $,
откуда $ M_4 = R_A x - P \cdot (x - a) - P \cdot (x - 2a) + R_B \cdot (x - 3a) = \frac{2}{3}Px - Px + Pa - Px + 2Pa + \frac{7}{3}Px - 7Pa = Px - 4Pa $.


\section{Задача 8}

$ \sum M_x = M_A + PL - q \cdot L \cdot \left(2L + \frac{L}{2}\right) - qL^2 = 0 $,
откуда $ M_A = -PL + 2qL^2 + \frac{1}{2}qL^2 + qL^2 = -2qL + \frac{7}{2}qL^2 = \frac{3}{2}qL^2 = \frac{3}{4}PL $.

$ \sum P_y = -R_A - P + qL = 0 $,
откуда $ R_A = -P + qL = -2qL + qL = -qL = -\frac{1}{2}P $.

\vspace{1.5ex}

Участок 1 $ \left(0 \le x < L\right) $

$ \sum P_{y_1} = R_A - Q_1 = 0 $,
откуда $ Q_1 = R_A = -\frac{1}{2}P $.

$ \sum M_{x_1} = -R_A x + M_A + M_1 = 0 $,
откуда $ M_1 = R_A x - M_A = -\frac{1}{2}Px - \frac{3}{4}PL $.

\vspace{1.5ex}

Участок 2 $ \left(L \le x < 2L\right) $

$ \sum P_{y_2} = R_A + P - Q_2 = 0 $,
откуда $ Q_2 = R_A + P = -\frac{1}{2}P + P = \frac{1}{2}P $.

$ \sum M_{x_2} = -R_A x + M_A - P(x - L) + M_2 = 0 $,
откуда $ M_2 = R_A x - M_A + P(x - L) = -\frac{1}{2}Px - \frac{3}{4}PL + Px - PL = \frac{1}{2}Px - \frac{7}{4}PL $.

\vspace{1.5ex}

Участок 3 $ \left(2L \le x < 3L\right) $

$ \sum P_{y_3} = R_A + P - q(x - 2L) - Q_3 = 0 $,
откуда $ Q_3 = R_A + P - q(x - 2L) = -\frac{1}{2}P + P - qx + 2qL = -\frac{x}{2L}P + \frac{3}{2}P $.

$ \sum M_{x_3} = -R_A x + M_A - P(x - L) - q(x - 2L) \cdot \frac{x-2L}{2} + M_3 = 0 $,
откуда $ M_3 = R_A x - M_A + P(x - L) + \frac{1}{2}q(x - 2L)^2 = -\frac{1}{2}Px - \frac{3}{4}PL + Px - PL - \frac{1}{2}q(x - 2L)^2 = -\frac{1}{2}q(x - 2L)^2 + \frac{1}{2}Px - \frac{7}{4}PL $.

\section{Задача 9}

$ \sum M_A = -M + 2M + R_B L = 0 $,
откуда $ R_B = -\frac{M}{L} = -P $.

$ \sum M_B = R_A L - M + 2M = 0 $,
откуда $ R_A = -\frac{M}{L} = -P $.

\vspace{1.5ex}

Участок 1 $ \left(0 \le x < \frac{L}{2}\right) $

$ Q_{y_1} = R_A - Q_1 = 0 $,
откуда $ Q_1 = R_A = -P $.

$ M_{x_1} = -M - R_A x + M_1 = 0 $,
откуда $ M_1 = M + R_A x = -Px + M $.

\vspace{1.5ex}

Участок 2 $ \left(\frac{L}{2} \le x < L\right) $

$ Q_{y_2} = R_A - Q_2 = 0 $,
откуда $ Q_2 = R_A = -P $.

$ M_{x_2} = -M - R_A x + 2M + M_2 = 0 $,
откуда $ M_2 = -M + R_A x = -Px - M $.

\section{Задача 10}

$ \sum M_A = -q \cdot 2L \cdot L + R_B \cdot 2L - qL^2 = 0 $,
откуда $ R_B = \frac{1}{2L}\left(2qL^2 + qL^2\right) = \frac{3}{2}P $.

$ \sum M_B = -R_A \cdot 2L + q \cdot 2L \cdot L - qL^2 = 0 $,
откуда $ R_A = \frac{1}{2L}\left(2qL^2 - qL^2\right) = \frac{1}{2}P $.

$ \sum P_y = R_A - q \cdot 2L + R_B = \frac{1}{2}P - 2P + \frac{3}{2}P = 0 $.

\vspace{1.5ex}

Участок 1 $ \left(0 \le x < 2L\right) $

$ \sum Q_{y_1} = R_A - qx - Q_1 = 0 $,
откуда $ Q_1 = R_A - qx = -\frac{x}{L}P + \frac{1}{2}P $.

$ \sum M_{x_1} = -R_A x + q \cdot x \cdot \frac{1}{2}x + M_1 = 0 $,
откуда $ M_1 = R_A x - \frac{1}{2}qx^2 = -\frac{1}{2}P \cdot \frac{x^2}{L} + \frac{1}{2}Px $.

\vspace{1.5ex}

Участок 2 $ \left(2L \le x < 3L\right) $

$ \sum Q_{y_2} = R_A - q \cdot 2L + R_B - Q_2 = 0 $,
откуда $ Q_2 = R_A - qx + R_B = -\frac{x}{L}P + 2P $.

$ \sum M_{x_2} = -R_A x + q \cdot 2L \cdot \frac{1}{2}(x - L) - R_B (x - 2L) + M_2 = 0 $,
откуда $ M_2 = R_A x - qL(x - L) + R_B (x - 2L) = \frac{1}{2}Px - Px + PL + \frac{3}{2}Px - 3PL = Px - 2PL $.


\section{Задача 11}

$ \sum M_A = -2q \cdot L \cdot 1.5L + R_B \cdot 3L - 3qL^2 = 0 $,
откуда $ R_B = \frac{1}{3L}\left(3qL^2 + 3qL^2\right) = 2P $.

$ \sum M_B = -R_A \cdot 3L + 2q \cdot L \cdot 1.5L - 3qL^2 = 0 $,
откуда $ R_A = \frac{1}{3L}\left(3qL^2 - 3qL^2\right) = 0 $.

$ \sum P_y = R_A - 2qL + R_B = 2P - 2P = 0 $.

\vspace{1.5ex}

Участок 1 $ \left(0 \le x < L\right) $

$ \sum Q_{y_1} = R_A - Q_1 = 0 $,
откуда $ Q_1 = R_A = 0 $.

$ \sum M_{x_1} = -R_A x + M_1 = 0 $,
откуда $ M_1 = R_A x = 0 $.

\vspace{1.5ex}

Участок 2 $ \left(L \le x < 2L\right) $

$ \sum Q_{y_2} = R_A - 2q(x - L) - Q_2 = 0 $,
откуда $ Q_2 = R_A - 2qx + 2qL = -2P\frac{x}{L} + 2P $.

$ \sum M_{x_2} = -R_A x + 2q \cdot (x - L) \cdot \frac{x-L}{2} + M_2 = 0 $,
откуда $ M_2 = R_A x - q(x - L)^2 = -q(x - L)^2 = -P\frac{x^2}{L} + 2Px - PL $.

\vspace{1.5ex}

Участок 3 $ \left(2L \le x < 3L\right) $

$ \sum Q_{y_3} = R_A - 2qL - Q_3 = 0 $,
откуда $ Q_3 = R_A - 2qL = -2P $.

$ \sum M_{x_3} = -R_A x + 2q \cdot L \cdot (x-1.5L) + M_3 = 0 $,
откуда $ M_3 = R_A x - 2qL(x - 1.5L) = -2Px + 3PL $.


\section{Задача 12}

$ \sum M_A = q \cdot L \cdot 0.5L - qL^2 + R_B \cdot 2L - q \cdot L \cdot 2.5L = 0 $,
откуда $ R_B = \frac{1}{2L}\left(-0.5qL^2 + qL^2 + 2.5qL^2\right) = 1.5qL = 1.5P $.

$ \sum M_B = -R_A \cdot 2L - q \cdot L \cdot 1.5L + qL \cdot L - q \cdot L \cdot 0.5L = 0 $,
откуда $ R_A = \frac{1}{2L}\left(-1.5qL^2 + qL^2 - 0.5qL^2\right) = -0.5P $.

$ \sum P_y = R_A + qL - qL + R_B - qL = -0.5P + 1.5P - P = 0 $

\vspace{1.5ex}

Участок 1 $ \left(0 \le x < L\right) $

$ \sum Q_{y_1} = R_A + qx - Q_1 = 0 $,
откуда $ Q_1 = R_A + qx = P\frac{x}{L} - 0.5P $.

$ \sum M_{x_1} = -R_A x - q \cdot x \cdot 0.5x + M_1 = 0 $,
откуда $ M_1 = R_A x + 0.5qx^2 = 0.5P\frac{x^2}{L} - 0.5Px $.

\vspace{1.5ex}

Участок 2 $ \left(L \le x < 2L\right) $

$ \sum Q_{y_2} = R_A + qL - qL - Q_2 = 0 $,
откуда $ Q_2 = R_A = -0.5P $.

$ \sum M_{x_2} = -R_A x - q \cdot L \cdot (x - 0.5L) + qL \cdot (x - L) + M_2 = 0 $,
откуда $ M_2 = R_A x + qL(x - 0.5L) - qL(x - L) = Px - 0.5Px - Px - 0.5PL + PL = -0.5Px + 0.5PL $.

\vspace{1.5ex}

Участок 3 $ \left(2L \le x < 3L\right) $

$ \sum Q_{y_3} = R_A + qL - qL - q(x - 2L) - Q_3 = 0 $,
откуда $ Q_3 = R_A - q(x - 2L) = -P\frac{x}{L} - 1.5P $.

$ \sum M_{x_3} = -R_A x - q \cdot L \cdot (x - 0.5L) + qL \cdot (x - L) - R_B (x - 2L) + q \cdot (x - 2L) \cdot \frac{x-2L}{2} + M_3 = 0 $,
откуда 
\begin{multline*}
    M_3 = R_A x + qL(x - 0.5L) - qL(x - L) + R_B (x - 2L) - 0.5q(x - 2L)^2 = \\
    = -0.5Px + Px - 0.5PL - Px + PL + 1.5Px - 3PL - 0.5P\frac{x^2}{L} + 2Px - 2PL = \\
    = -0.5P\frac{x^2}{L} + 3Px - 4.5PL 
\end{multline*}.


















